refactor: Merge GraphAux with conformance

src/GraphConformance.v
@@ -14,7 +14,6 @@ Require Import Schema.
 Require Import SchemaWellFormedness.
 Require Import SchemaAux.
 Require Import Graph.
-Require Import GraphAux.
 
 (* end hide *)
 
@@ -49,7 +48,61 @@ Section Conformance.
 
   Variables (Vals: eqType).
 
+  Section GraphAux.
+
+    Variable (graph :  @graphQLGraph Vals).
+    Implicit Type edge : @node Vals * @fld Vals * @node Vals.
+
+    
+    
+    (** Extractors for an edge **)
+
+
+    Definition etarget edge : node :=
+      let: (_, _, v) := edge in v.
+
+    Definition esource edge : node :=
+      let: (u, _, _) := edge in u.
+
+    Definition efield edge : fld :=
+      let: (_, f, _) := edge in f.
+
+    Definition enodes edge : seq node := [:: edge.(esource) ; edge.(etarget)].
+    
+    (** Get all nodes from a graph **)
+    Definition nodes graph : seq node :=
+      undup (graph.(root) ::  flatten [seq edge.(enodes) | edge <- graph.(E)]).
+
+
+
+    (** Get all neighbours of a node irrespective of the field in the edge 
+      connecting the two **)
+    Definition neighbours (u : node) (edges : seq (node * fld * node)) : seq node :=
+      undup [seq edge.(etarget) | edge <- edges & edge.(esource) == u]. 
+
+    
+
+
+    (** Get all neighbours of a node that are linked via an edge with a given
+      field. **)
+    Definition neighbours_with_field (u : node) (f : fld) : seq node :=
+      undup [seq edge.(etarget) |  edge <- [seq edge <- graph.(E) | (esource edge == u) & (efield edge == f)]].
+
+
+    (** 
+      Checks whether there is only one edge coming out of the source node and 
+      having the given field.
+     **)
+    Definition is_field_unique_for_src_node graph (src_node : node) (f : fld) : bool :=
+      uniq [seq edge <- graph.(E) | (esource edge == src_node) & (efield edge == f)].
+    
+    
+    
+
+  End GraphAux.
+
   
+
   Implicit Type schema : @wfGraphQLSchema Vals.
   Implicit Type graph : @graphQLGraph Vals. 
 
@@ -185,7 +238,7 @@ Section Conformance.
 
 End Conformance.
 
-Arguments conformedGraph [Vals].
+
 
 (** ---- *)
 (** 
