src/theory/GraphConformanceLemmas.v
@@ -11,9 +11,8 @@ Require Import QString.
 Require Import Schema.
 Require Import SchemaWellFormedness.
 Require Import SchemaAux.
-Require Import Graph.
-Require Import GraphAux.
 
+Require Import Graph.
 Require Import GraphConformance.
 
 Require Import SeqExtra.
@@ -25,10 +24,51 @@ Section Theory.
 
   Variables (Vals: eqType).
 
+  Section Aux.
+
+    Variable (graph :  @graphQLGraph Vals).
+    Implicit Type edge : @node Vals * @fld Vals * @node Vals.
+
+  
+
+    Lemma root_in_nodes : graph.(root) \in graph.(nodes).
+    Proof.
+      rewrite /nodes -in_undup.
+        by apply/orP; left; apply/eqP.
+    Qed.
+
+    
+    Lemma neighbours_are_in_nodes u fld:
+      forall x, x \in neighbours_with_field graph u fld -> x \in graph.(nodes).
+    Proof.
+      rewrite /neighbours_with_field /nodes => x.
+      rewrite -?in_undup => /mapP [v].
+      rewrite mem_filter => /andP [/andP [/eqP Hsrc /eqP Hfld] Hin] /= Heq.
+      apply/orP; right.
+      apply/flatten_mapP.
+      exists v => //=.
+      rewrite /enodes inE; apply/orP; right.
+        by rewrite mem_seq1; apply/eqP.
+    Qed.
+    
+    
+    
+    Lemma ohead_in_nodes nds v :
+      all (fun node => node \in graph.(nodes)) nds ->
+      ohead nds = Some v ->
+      v \in graph.(nodes). 
+    Proof.
+      elim: nds => // x nds IH /=.
+        by move=> H; case=> Heq; rewrite Heq in H; move/andP: H => [H _]. 
+    Qed.
+  
+
+  End Aux.
+
+
   Variable (s : @wfGraphQLSchema Vals) (g : conformedGraph s).
 
-
-
+    
   (**
      This lemma states that if the root node's type conforms to the schema, 
      then its type must be the Query type.
